\documentclass[11pt,a4paper]{article}
\usepackage[latin1]{inputenc}
\usepackage{amsmath}
\usepackage{amsfonts}
\usepackage{amssymb}
\begin{document}

It is obvious therefore that, $R_{\mu \nu} -\frac{1}{2}g_{\mu \nu} R = -\kappa   T_{\mu \nu} = G_{\mu \nu} $ \ldots.

or use,

\begin{gather}
\begin{aligned}
\therefore \;R_{\mu \nu} -\frac{1}{2}g_{\mu \nu} R &= -\kappa        T_{\mu \nu}\\
& = G_{\mu \nu} 
\end{aligned}
\end{gather}

\begin{equation}
\begin{aligned}
\therefore \;R_{\mu \nu} -\frac{1}{2}g_{\mu \nu} R &= -\kappa        T_{\mu \nu}\\
& = G_{\mu \nu} 
\end{aligned}
\end{equation}



\begin{align}
\therefore \;R_{\mu \nu} -\frac{1}{2}g_{\mu \nu} R &= -\kappa        T_{\mu \nu}\\
& = G_{\mu \nu} 
\end{align}

\[
\begin{aligned}
\therefore \;R_{\mu \nu} -\frac{1}{2}g_{\mu \nu} R &= -\kappa        T_{\mu \nu}\\
& = G_{\mu \nu} 
\end{aligned}
\]

\begin{align*}
\therefore \;R_{\mu \nu} -\frac{1}{2}g_{\mu \nu} R &= -\kappa        T_{\mu \nu}\\
& = G_{\mu \nu} 
\end{align*}


\end{document}